<https://data.vlaanderen.be/ns/FeitelijkeVerenigingen> a <http://www.w3.org/2002/07/owl#Ontology>.
<https://data.vlaanderen.be/ns/FeitelijkeVerenigingen#FeitelijkeVereniging> a <http://www.w3.org/2002/07/owl#Class>;
    <http://www.w3.org/2000/01/rdf-schema#isDefinedBy> <https://data.vlaanderen.be/ns/FeitelijkeVerenigingen>;
    <http://www.w3.org/2000/01/rdf-schema#comment> "An Association without legal personality, based on an agreement between two or more persons and/or organisations to pursue a selfless purpose within the framework of one or more well-defined activities."@en;
    <http://www.w3.org/2000/01/rdf-schema#subClassOf> <https://data.vlaanderen.be/ns/FeitelijkeVerenigingen#Vereniging>;
    <http://purl.org/vocab/vann/usageNote> "An Association is an Organization that pursues a selfless goal. This also applies to a de facto association, only it does not have legal personality: the individual members of the de facto association may be liable."@en.
<https://data.vlaanderen.be/ns/FeitelijkeVerenigingen#Erkenningsaanvraag> a <http://www.w3.org/2002/07/owl#Class>;
    <http://www.w3.org/2000/01/rdf-schema#isDefinedBy> <https://data.vlaanderen.be/ns/FeitelijkeVerenigingen>;
    <http://www.w3.org/2000/01/rdf-schema#comment> "The request for designation by a competent institution establishing that a person or institution meets certain requirements, whether temporary or not."@en;
    <http://www.w3.org/2000/01/rdf-schema#subClassOf> <http://purl.org/vocab/cpsv#PublicService>.
<https://data.vlaanderen.be/ns/FeitelijkeVerenigingen#Erkenning> a <http://www.w3.org/2002/07/owl#Class>;
    <http://www.w3.org/2000/01/rdf-schema#isDefinedBy> <https://data.vlaanderen.be/ns/FeitelijkeVerenigingen>;
    <http://www.w3.org/2000/01/rdf-schema#comment> "The designation by a competent institution establishing that a person or institution meets certain requirements, whether temporary or not."@en;
    <http://www.w3.org/2000/01/rdf-schema#subClassOf> <https://data.europa.eu/m8g/Output>.
<https://data.vlaanderen.be/ns/FeitelijkeVerenigingen#Vereniging> a <http://www.w3.org/2002/07/owl#Class>;
    <http://www.w3.org/2000/01/rdf-schema#isDefinedBy> <https://data.vlaanderen.be/ns/FeitelijkeVerenigingen>;
    <http://www.w3.org/2000/01/rdf-schema#comment> "An Organization that pursues a selfless goal."@en;
    <http://www.w3.org/2000/01/rdf-schema#subClassOf> <http://www.w3.org/ns/org#Organization>.
<https://data.vlaanderen.be/ns/FeitelijkeVerenigingen#bankrekeningnummer> a <http://www.w3.org/2002/07/owl#DatatypeProperty>;
    <http://www.w3.org/2000/01/rdf-schema#isDefinedBy> <https://data.vlaanderen.be/ns/FeitelijkeVerenigingen>;
    <http://www.w3.org/2000/01/rdf-schema#domain> <https://data.vlaanderen.be/ns/FeitelijkeVerenigingen#FeitelijkeVereniging>;
    <http://www.w3.org/2000/01/rdf-schema#range> <http://www.w3.org/2000/01/rdf-schema#Literal>;
    <http://www.w3.org/2000/01/rdf-schema#comment> "A unique number assigned to an account at a bank."@en.
<https://data.vlaanderen.be/ns/FeitelijkeVerenigingen#Persoon.geboortedatum> a <http://www.w3.org/2002/07/owl#DatatypeProperty>;
    <http://www.w3.org/2000/01/rdf-schema#isDefinedBy> <https://data.vlaanderen.be/ns/FeitelijkeVerenigingen>;
    <http://www.w3.org/2000/01/rdf-schema#domain> <http://www.w3.org/ns/person#Person>;
    <http://www.w3.org/2000/01/rdf-schema#range> <http://www.w3.org/2001/XMLSchema#dateTime>;
    <http://www.w3.org/2000/01/rdf-schema#comment> "Date of birth."@en.
<https://data.vlaanderen.be/ns/FeitelijkeVerenigingen#geldigheidsperiodeErkenning> a <http://www.w3.org/2002/07/owl#ObjectProperty>;
    <http://www.w3.org/2000/01/rdf-schema#isDefinedBy> <https://data.vlaanderen.be/ns/FeitelijkeVerenigingen>;
    <http://www.w3.org/2000/01/rdf-schema#domain> <https://data.vlaanderen.be/ns/FeitelijkeVerenigingen#Erkenningsaanvraag>;
    <http://www.w3.org/2000/01/rdf-schema#range> <http://data.europa.eu/m8g/PeriodOfTime>;
    <http://www.w3.org/2000/01/rdf-schema#comment> "Time interval, stated in the application for recognition, for which the approval that has been applied for will apply."@en;
    <http://purl.org/vocab/vann/usageNote> "The time interval to which the validity period of an Application for Recognition is entitled may differ from the Recognition that is finally granted."@en.
<https://data.vlaanderen.be/ns/FeitelijkeVerenigingen#Erkenningsaanvraag.activiteit> a <http://www.w3.org/2002/07/owl#ObjectProperty>;
    <http://www.w3.org/2000/01/rdf-schema#isDefinedBy> <https://data.vlaanderen.be/ns/FeitelijkeVerenigingen>;
    <http://www.w3.org/2000/01/rdf-schema#domain> <https://data.vlaanderen.be/ns/FeitelijkeVerenigingen#Erkenningsaanvraag>;
    <http://www.w3.org/2000/01/rdf-schema#range> <http://www.w3.org/2004/02/skos/core#Concept>;
    <http://www.w3.org/2000/01/rdf-schema#comment> "Type of activity carried out by an organization."@en.
<https://data.vlaanderen.be/ns/FeitelijkeVerenigingen#Erkenning.activiteit> a <http://www.w3.org/2002/07/owl#ObjectProperty>;
    <http://www.w3.org/2000/01/rdf-schema#isDefinedBy> <https://data.vlaanderen.be/ns/FeitelijkeVerenigingen>;
    <http://www.w3.org/2000/01/rdf-schema#domain> <https://data.vlaanderen.be/ns/FeitelijkeVerenigingen#Erkenning>;
    <http://www.w3.org/2000/01/rdf-schema#range> <http://www.w3.org/2004/02/skos/core#Concept>;
    <http://www.w3.org/2000/01/rdf-schema#comment> "Type of activity carried out by an organization."@en.
<https://data.vlaanderen.be/ns/FeitelijkeVerenigingen#geldigheidsperiode> a <http://www.w3.org/2002/07/owl#ObjectProperty>;
    <http://www.w3.org/2000/01/rdf-schema#isDefinedBy> <https://data.vlaanderen.be/ns/FeitelijkeVerenigingen>;
    <http://www.w3.org/2000/01/rdf-schema#domain> <https://data.vlaanderen.be/ns/FeitelijkeVerenigingen#Erkenning>;
    <http://www.w3.org/2000/01/rdf-schema#range> <http://data.europa.eu/m8g/PeriodOfTime>;
    <http://www.w3.org/2000/01/rdf-schema#comment> "Time interval within which the recognition applies."@en.
<https://data.vlaanderen.be/ns/FeitelijkeVerenigingen#Persoon.woonplaats> a <http://www.w3.org/2002/07/owl#ObjectProperty>;
    <http://www.w3.org/2000/01/rdf-schema#isDefinedBy> <https://data.vlaanderen.be/ns/FeitelijkeVerenigingen>;
    <http://www.w3.org/2000/01/rdf-schema#domain> <http://www.w3.org/ns/person#Person>;
    <http://www.w3.org/2000/01/rdf-schema#range> <http://purl.org/dc/terms/Location>;
    <http://www.w3.org/2000/01/rdf-schema#comment> "Place where a person lives."@en.
<https://data.vlaanderen.be/ns/FeitelijkeVerenigingen#toegekenddoor> a <http://www.w3.org/2002/07/owl#ObjectProperty>;
    <http://www.w3.org/2000/01/rdf-schema#isDefinedBy> <https://data.vlaanderen.be/ns/FeitelijkeVerenigingen>;
    <http://www.w3.org/2000/01/rdf-schema#domain> <https://data.vlaanderen.be/ns/FeitelijkeVerenigingen#Erkenning>;
    <http://www.w3.org/2000/01/rdf-schema#range> <http://data.europa.eu/m8g/PublicOrganisation>;
    <http://www.w3.org/2000/01/rdf-schema#comment> "Reference to the organisation that granted the recognition to the de facto association."@en.
<https://data.vlaanderen.be/ns/FeitelijkeVerenigingen#heeftErkenning> a <http://www.w3.org/2002/07/owl#ObjectProperty>;
    <http://www.w3.org/2000/01/rdf-schema#isDefinedBy> <https://data.vlaanderen.be/ns/FeitelijkeVerenigingen>;
    <http://www.w3.org/2000/01/rdf-schema#domain> <https://data.vlaanderen.be/ns/FeitelijkeVerenigingen#FeitelijkeVereniging>;
    <http://www.w3.org/2000/01/rdf-schema#range> <https://data.vlaanderen.be/ns/FeitelijkeVerenigingen#Erkenning>;
    <http://www.w3.org/2000/01/rdf-schema#comment> "Reference to the recognition(s) that the de facto association has."@en.
<https://data.vlaanderen.be/ns/FeitelijkeVerenigingen#geeftrechtOp> a <http://www.w3.org/2002/07/owl#ObjectProperty>;
    <http://www.w3.org/2000/01/rdf-schema#isDefinedBy> <https://data.vlaanderen.be/ns/FeitelijkeVerenigingen>;
    <http://www.w3.org/2000/01/rdf-schema#domain> <https://data.vlaanderen.be/ns/FeitelijkeVerenigingen#Erkenningsaanvraag>;
    <http://www.w3.org/2000/01/rdf-schema#range> <https://data.vlaanderen.be/ns/FeitelijkeVerenigingen#Erkenning>;
    <http://www.w3.org/2000/01/rdf-schema#comment> "The recognition that is granted on the basis of the submitted application for recognition."@en.
<https://data.vlaanderen.be/ns/FeitelijkeVerenigingen#dientIn> a <http://www.w3.org/2002/07/owl#ObjectProperty>;
    <http://www.w3.org/2000/01/rdf-schema#isDefinedBy> <https://data.vlaanderen.be/ns/FeitelijkeVerenigingen>;
    <http://www.w3.org/2000/01/rdf-schema#domain> <https://data.vlaanderen.be/ns/FeitelijkeVerenigingen#FeitelijkeVereniging>;
    <http://www.w3.org/2000/01/rdf-schema#range> <https://data.vlaanderen.be/ns/FeitelijkeVerenigingen#Erkenningsaanvraag>;
    <http://www.w3.org/2000/01/rdf-schema#comment> "The application for recognition submitted by the de facto association."@en.
<https://data.vlaanderen.be/ns/FeitelijkeVerenigingen#vraagtAan> a <http://www.w3.org/2002/07/owl#ObjectProperty>;
    <http://www.w3.org/2000/01/rdf-schema#isDefinedBy> <https://data.vlaanderen.be/ns/FeitelijkeVerenigingen>;
    <http://www.w3.org/2000/01/rdf-schema#domain> <https://data.vlaanderen.be/ns/FeitelijkeVerenigingen#FeitelijkeVereniging>;
    <http://www.w3.org/2000/01/rdf-schema#range> <http://purl.org/vocab/cpsv#PublicService>;
    <http://www.w3.org/2000/01/rdf-schema#comment> "Reference to the public service requested by the de facto association."@en.
<https://data.vlaanderen.be/ns/FeitelijkeVerenigingen#heeftLid> a <http://www.w3.org/2002/07/owl#ObjectProperty>;
    <http://www.w3.org/2000/01/rdf-schema#isDefinedBy> <https://data.vlaanderen.be/ns/FeitelijkeVerenigingen>;
    <http://www.w3.org/2000/01/rdf-schema#domain> <https://data.vlaanderen.be/ns/FeitelijkeVerenigingen#FeitelijkeVereniging>;
    <http://www.w3.org/2000/01/rdf-schema#range> <http://purl.org/dc/terms/Agent>;
    <http://www.w3.org/2000/01/rdf-schema#comment> "Reference to the members who are part of the de facto association."@en.
<https://data.vlaanderen.be/ns/FeitelijkeVerenigingen#heeftVertegenwoordiger> a <http://www.w3.org/2002/07/owl#ObjectProperty>;
    <http://www.w3.org/2000/01/rdf-schema#isDefinedBy> <https://data.vlaanderen.be/ns/FeitelijkeVerenigingen>;
    <http://www.w3.org/2000/01/rdf-schema#domain> <https://data.vlaanderen.be/ns/FeitelijkeVerenigingen#FeitelijkeVereniging>;
    <http://www.w3.org/2000/01/rdf-schema#range> <http://purl.org/dc/terms/Agent>;
    <http://www.w3.org/2000/01/rdf-schema#comment> "Reference to the representative of the de facto association."@en.
<https://data.vlaanderen.be/ns/FeitelijkeVerenigingen#isPositieIn> a <http://www.w3.org/2002/07/owl#ObjectProperty>;
    <http://www.w3.org/2000/01/rdf-schema#isDefinedBy> <https://data.vlaanderen.be/ns/FeitelijkeVerenigingen>;
    <http://www.w3.org/2000/01/rdf-schema#domain> <http://purl.org/dc/terms/Agent>;
    <http://www.w3.org/2000/01/rdf-schema#range> <https://data.vlaanderen.be/ns/FeitelijkeVerenigingen#FeitelijkeVereniging>;
    <http://www.w3.org/2000/01/rdf-schema#comment> "The representative is a position in the de facto association."@en.
